\begin{flushright}
\large
\setlength{\abovedisplayskip}{10pt}
\setlength{\belowdisplayskip}{10pt}

$$
\binom{n}{k} = \binom{n}{n-k}
$$

$$
\binom{n}{k} = \frac{n}{k}\binom{n-1}{k-1}, \quad (1 \le k \le n)
$$

$$
\sum_{k=0}^{n} \binom{n}{k} = 2^{n}
$$

$$
\sum_{m=0}^{n} \binom{m}{k} = \binom{n+1}{k+1}, \quad (n \ge k \ge 0)
$$

$$
\sum_{k=0}^{m} \binom{n+k}{k} = \binom{n+m+1}{m}
$$

$$
\binom{n}{0}^2 + \binom{n}{1}^2 + \cdots + \binom{n}{n}^2 = \binom{2n}{n}
$$

$$
\sum_{k=1}^{n} k\binom{n}{k} = n2^{n-1}
$$

$$
F_n = \sum_{k=0}^{\lfloor\frac{n-1}{2}\rfloor} \binom{n-k-1}{k}
$$

$$
F_{n+1} = \sum_{k=0}^{\lfloor \frac{n}{2} \rfloor} \binom{n-k}{k}
$$
\end{flushright}
